Add RSA memory invariants

impl/riscv/rsa_ops.i.dfy
@@ -17,9 +17,10 @@ module rsa_ops {
     import opened BASE_32_Seq
     import opened Seq
 
-    function to_nat(xs: seq<uint32>): nat
+    function ToNat(xs: seq<BASE_32_Seq.uint>): nat
     {
-        ToNatRight(xs)
+        assert BASE() == BASE_32;
+        BASE_32_Seq.ToNatRight(xs)
     }
 
     function seq_subb(xs: seq<uint32>, ys: seq<uint32>): (seq<uint32>, uint1)
@@ -43,5 +44,101 @@ module rsa_ops {
         ensures ToNatRight(xs) == xs[0] + xs[1] * BASE_32
     {
         LemmaSeqLen2(xs);
+    }
+
+    /* rsa/mm definions & lemmas */
+   datatype rsa_params = rsa_params(
+        M: nat, 
+        M0D: uint,
+        R: nat,
+        RR: nat,
+        R_INV: nat,
+        E: nat,
+        E0: uint32,
+        SIG: nat,
+        B32_INV: nat)
+
+    predicate rsa_params_inv(rsa: rsa_params)
+    {
+        // E0 is derived from the exponent E
+        && rsa.E == Pow(2, rsa.E0) + 1
+
+        // modulo is none zero
+        && rsa.M != 0
+        && cong_B32(rsa.M0D * rsa.M, -1)
+
+        // signature
+        && 0 < rsa.SIG < rsa.M
+
+        && rsa.R == Pow(BASE_32, NUM_WORDS)
+
+        && rsa.RR < rsa.M
+        && IsModEquivalent(rsa.RR, rsa.R * rsa.R, rsa.M)
+
+        && rsa.R_INV == Pow(rsa.B32_INV, NUM_WORDS)
+        && IsModEquivalent(rsa.R_INV * rsa.R, 1, rsa.M)
+
+        && IsModEquivalent(BASE_32 * rsa.B32_INV, 1, rsa.M)
+    }
+
+    datatype mvars = mvars(
+        x_it: iter_t,
+        y_it: iter_t,
+
+        m_it: iter_t,
+        rr_it: iter_t,
+        sig_it: iter_t,
+        rsa: rsa_params)
+
+    predicate mvars_iter_init(iter: iter_t, mem: mem_t, address: int, value: int)
+    {
+        && (address >= 0 ==> iter_inv(iter, mem, address))
+        && (value >= 0 ==> ToNat(iter.buff) == value)
+        && iter.index == 0
+        && |iter.buff| == NUM_WORDS
+    }
+
+    predicate m0d_it_inv(iter: iter_t, mem: mem_t, address: int)
+    {
+        && (address >= 0 ==> iter_inv(iter, mem, address))
+        && iter.index == 0
+        && |iter.buff| == 1
+    }
+
+    predicate mvars_inv(
+        vars: mvars,
+        mem: mem_t,
+        x_ptr: int,
+        y_ptr: int,
+        m_ptr: int,
+        rr_ptr: int,
+        sig_ptr: int)
+    {
+        && rsa_params_inv(vars.rsa)
+
+        && mvars_iter_init(vars.x_it, mem, x_ptr, NA)
+        && mvars_iter_init(vars.y_it, mem, y_ptr, NA)
+        && mvars_iter_init(vars.sig_it, mem, sig_ptr, vars.rsa.SIG)
+        && mvars_iter_init(vars.m_it, mem, m_ptr, vars.rsa.M)
+        && mvars_iter_init(vars.rr_it, mem, rr_ptr, vars.rsa.RR)
+    }
+
+    predicate mvars_init(
+        vars: mvars,
+        mem: mem_t,
+        m_ptr: uint32,
+        rr_ptr: uint32,
+        sig_ptr: uint32,
+        out_ptr: uint32)
+    {
+        && rsa_params_inv(vars.rsa)
+
+        && mvars_inv(vars, mem, NA, NA, m_ptr, rr_ptr, sig_ptr)
+        && out_ptr in mem
+        && |mem[out_ptr]| == NUM_WORDS
+
+        && out_ptr != rr_ptr
+        && out_ptr != m_ptr
+        && out_ptr != sig_ptr
     }
 }
